Migrate from coq-prelude to coq-ext-lib
Since its initial release, coq-comparse was using coq-prelude, a
home-grown, “opinionated” prelude library for Coq. This library was
published as an open source project, but never made available as an
OPAM package. In the meantime, the ExtLib coq project became more and
more popular, and often exceeds the scope of coq-prelude.

As a consequence, we take the decision to move away from coq-prelude,
in order to adopt coq-ext-lib instead.

theories/Combinators.v
@@ -1,9 +1,14 @@
-From Coq Require Import String FunInd Recdef.
-From Prelude Require Import All Text.
+From Coq Require Import String FunInd Recdef List.
+From ExtLib Require Import RelDec.
 From Comparse Require Import Monad.
 
-#[local]
-Open Scope text_scope.
+Import ListNotations.
+Import MonadLetNotation.
+
+Generalizable All Variables.
+
+Open Scope parser_scope.
+Open Scope monad_scope.
 
 (** ** <<many>> *)
 
@@ -14,36 +19,38 @@ Open Scope text_scope.
         succeeds at least once.
       - [many p] never fails. *)
 
-(* begin hide *)
 Function many_aux (i t : Type) (I : Input i t) (α : Type) (p : parser i α) (S : StrictParser p)
     (input : i) (acc : list α) {measure length input}
   : list α * i :=
-  match p input with
-  | inl _ => (rev acc, input)
+  match runStateT p input with
   | inr (x, output) => many_aux i t I α p S output (x :: acc)
+  | inl _ => (rev acc, input)
   end.
 
 Proof.
   intros i t I a p S input acc res x output eqr equ.
   now apply is_strict in equ.
 Defined.
-(* end hide *)
+
+Arguments many_aux {_ _ _ _} _ [_] _ _.
+
 Definition many `{Input i t} {α} (p : parser i α) `{StrictParser i t α p} : parser i (list α) :=
-  fun (input : i) => inr (many_aux _ _ _ _ p _ input []).
+  mkStateT (fun (input : i) => inr (many_aux p input [])).
 
 Instance many_parser `(StrictParser i t α p) : Parser (many p).
-(* begin hide *)
+
 Proof.
   unfold many.
   constructor.
   intros input x output equ.
-  functional induction (many_aux i t H α p H0 input []).
-  + now inversion equ; ssubst.
+  cbn in equ.
+  inversion equ.
+  functional induction (many_aux p input []).
   + transitivity (length output0).
-    ++ apply (IHp0 equ).
+    ++ eapply IHp0; eauto.
     ++ now apply is_parser in e.
+  + now inversion equ.
 Qed.
-(* end hide *)
 
 (** ** <<some>> *)
 
@@ -67,38 +74,41 @@ Definition some `{Input i t} {α} (p : parser i α) `{StrictParser i t α p} : p
       - [p <|> q] fails if both [p] and [q] fail. *)
 
 Definition alt `{Input i t} {α} (p q : parser i α) : parser i α :=
-  fun* input =>
-    match p input with
-    | inl _ => q input
-    | x => x
-    end.
+  mkStateT (fun input =>
+              match runStateT p input with
+              | inl _ => runStateT q input
+              | x => x
+              end).
 
-Infix "<|>" := alt (at level 50, left associativity) : monad_scope.
+Infix "<|>" := alt (at level 50, left associativity) : parser_scope.
 
-Instance alt_Parser `(Input i t, !@Parser i t α _ p, !@Parser i t α _  q) : @Parser i t α _ (alt p q).
-(* begin hide *)
+Instance alt_Parser `(Input i t, !@Parser i t α _ p, !@Parser i t α _  q)
+  : @Parser i t α _ (alt p q).
+
 Proof.
   unfold alt.
   constructor.
   intros input x output equ.
-  case_eq (p input).
+  case_eq (runStateT p input).
   + intros e eque.
+    cbn in equ.
     rewrite eque in equ.
     now apply is_parser in equ.
   + intros [x' output'] equ'.
+    cbn in equ.
     rewrite equ' in equ.
     inversion equ; subst.
     now apply is_parser in equ'.
 Qed.
-(* end hide *)
 
-Instance alt_Strict `(Input i t, !@StrictParser i t α _ p, !@StrictParser i t α _  q) : @StrictParser i t α _ (alt p q).
-(* begin hide *)
+Instance alt_Strict `(Input i t, !@StrictParser i t α _ p, !@StrictParser i t α _  q)
+  : @StrictParser i t α _ (alt p q).
+
 Proof.
   unfold alt.
   constructor.
   intros input x output equ.
-  case_eq (p input).
+  case_eq (runStateT p input); cbn in equ.
   + intros e eque.
     rewrite eque in equ.
     now apply is_strict in equ.
@@ -107,7 +117,6 @@ Proof.
     inversion equ; subst.
     now apply is_strict in equ'.
 Qed.
-(* end hide *)
 
 (** ** <<optional>> *)
 
@@ -123,8 +132,8 @@ Definition optional `{Input i t} {α} (p : parser i α) : parser i (option α) :
 
 (** ** <<fail>> *)
 
-Definition fail {i α} (msg : text) : parser i α :=
-  fun s => inl [msg].
+Definition fail {i α} (msg : string) : parser i α :=
+  mkStateT (fun s => inl [msg]).
 
 Instance fail_Parser `(Input i t) : Parser (@fail i α msg).
 
@@ -136,11 +145,11 @@ Qed.
 (** ** <<read_token>> *)
 
 Definition read_token `{Input i t} : parser i t :=
-  do let* input := get in
-     match unpack input with
-     | Some (x, rst) => put rst *> pure x
-     | None => fail "expected character, found end of input"
-     end
+  let* input := MonadState.get in
+  match unpack input with
+  | Some (x, rst) => put rst;;
+                     pure x
+  | None => fail "expected character, found end of input"
   end.
 
 Instance read_token_Strict : StrictParser (@read_token i t H).
@@ -153,8 +162,9 @@ Proof.
   case_eq (unpack input).
   + intros [y rst] equ'.
     rewrite equ' in equ.
+    cbn in equ.
     inversion equ; subst.
-    rewrite (unpack_length input output y equ').
+    rewrite (unpack_length input output x equ').
     auto.
   + intros equ'.
     now rewrite equ' in equ.
@@ -163,51 +173,56 @@ Qed.
 (** ** <<ensure>> *)
 
 Definition ensure `{Input i t} {α} (p : parser i α) (cond : α -> bool) : parser i α :=
-  do let* res := p in
-     if cond res
-     then pure res
-     else fail "ensure: result of p is not valid according to cond"
-  end.
+  let* res := p in
+  if cond res
+  then pure res
+  else fail "ensure: result of p is not valid according to cond".
 
 (** ** <<token>> *)
 
-Definition token `{EquDec t, I : Input i t} (a : t) : parser i t :=
-  ensure read_token (equalb a).
+Definition token `{RelDec t eqv, I : Input i t} (a : t) : parser i t :=
+  ensure read_token (rel_dec a).
 
 (** ** <<tag>> *)
 
-Function tag_aux (i t : Type) (Eq : Equality t) (E : @EquDec t Eq) (I : Input i t) (x : i) (input : i) {measure length x}
+Function tag_aux (i t : Type) (eqv : t -> t -> Prop) (H : @RelDec t eqv)
+    (I : Input i t) (x : i) (input : i)
+    {measure length x}
   : error_stack + (unit * i) :=
   match unpack input, unpack x with
   | Some (c, rst), Some (c', rst') =>
-    if equalb c c'
-    then tag_aux i t Eq E I rst' rst
-    else inl ["nop"]
+    if rel_dec c c'
+    then tag_aux i t _ H I rst' rst
+    else inl ["nop"%string]
   | _, None => inr (tt, input)
-  | _, _ => inl ["nop"]
+  | _, _ => inl ["nop"%string]
   end.
 
 Proof.
-  intros i t Eq E I x input [x' input'] c' rst' equ1 equ2 [y rst] y' rst'' equ3 equ4 equ5.
+  intros i t H' H I x input [x' input'] c' rst' equ1 equ2 [y rst] y' rst'' equ3 equ4 equ5.
   inversion equ3; subst.
   apply unpack_length in equ4.
   rewrite equ4.
   auto with arith.
 Defined.
 
-Definition tag `{E : EquDec t, I : Input i t} (x : i) : parser i unit :=
-  @tag_aux i t _ E I x.
+Arguments tag_aux [_ _ _ _ _] _ _.
 
-Instance tag_parser `(EquDec t, Input i t) : Parser (tag x).
-(* begin hide *)
+Definition tag `{RelDec t eqv, Input i t} (x : i) : parser i unit :=
+  mkStateT (fun input => tag_aux x input).
+
+Instance tag_parser `(RelDec t eqv, Input i t) : Parser (tag x).
+
 Proof.
   intros x.
   constructor.
   intros input r output equ.
   unfold tag in equ.
-  functional induction (tag_aux i t H H0 H1 x input).
+  cbn in *.
+  functional induction (tag_aux x input).
   + transitivity (length rst).
-    ++ now apply IHs.
+    ++ apply IHs.
+       apply equ.
     ++ apply unpack_length in e.
        rewrite e.
        auto with arith.
@@ -216,13 +231,13 @@ Proof.
     auto with arith.
   + discriminate.
 Qed.
-(* end hide *)
 
 (** [tag' x] is a variant of [tag x] which returns [x] and not [tt]. This can be
     useful used in conjunction of [<|>]. *)
 
-Definition tag' `{EquDec t, Input i t} (x : i) : parser i i :=
-  tag x *> pure x.
+Definition tag' `{RelDec t eqv, Input i t} (x : i) : parser i i :=
+  tag x;;
+  pure x.
 
 (** ** <<many_until>> *)
 
@@ -232,14 +247,13 @@ Definition tag' `{EquDec t, Input i t} (x : i) : parser i i :=
       - [many_until p q] is a _strict_ parser if _q_ is strict.
       - [many_until p q] fails if [p] fails before [q] could suceed. *)
 
-(* begin hide *)
 Function many_until_aux (α β i t : Type) (I : Input i t)
     (p : parser i α) (H : StrictParser p) (q : parser i β)
     (input : i) (acc : list α) {measure length input}
   : error_stack + (list α * i) :=
-  match q input with
-  | inl _ => match p input with
-             | inl _ => inl ["p failed before q could succeed"]
+  match runStateT q input with
+  | inl _ => match runStateT p input with
+             | inl _ => inl ["p failed before q could succeed"%string]
              | inr (x, output) => many_until_aux α β i t I p H q output (x :: acc)
              end
   | inr (_, output) => inr (rev acc, output)
@@ -249,20 +263,23 @@ Proof.
   intros α b i t I p H q input acc e eque res x output equr equ.
   now apply is_strict in equ.
 Defined.
-(* end hide *)
+
+Arguments many_until_aux [_ _ _ _ _] _ [_] _ _ _.
+
 Definition many_until {α β} `{Input i t}
     (p : parser i α) `{StrictParser i t α p} (q : parser i β)
   : parser i (list α) :=
-  fun input => many_until_aux _ _ _ _ _ p _ q input [].
+  mkStateT (fun input => many_until_aux p q input []).
 
 Instance many_until_parser `(Input i t, !StrictParser (p : parser i a), !Parser (q : parser i b))
   : Parser (many_until p q).
-(* begin hide *)
+
 Proof.
   constructor.
   intros input x output equ.
   unfold many_until in *.
-  functional induction (many_until_aux a b i t _ p _ q input []).
+  cbn in *.
+  functional induction (many_until_aux p q input []).
   + discriminate.
   + destruct many_until_aux.
     ++ discriminate.
@@ -274,16 +291,16 @@ Proof.
   + inversion equ; subst.
     now apply is_parser in e.
 Qed.
-(* end hide *)
 
 Instance many_until_strict `(Input i t, !StrictParser (p : parser i α), !StrictParser (q : parser i β))
   : StrictParser (many_until p q).
-(* begin hide *)
+
 Proof.
   constructor.
   intros input x output equ.
   unfold many_until in *.
-  functional induction (many_until_aux α β i t _ p _ q input []).
+  cbn in *.
+  functional induction (many_until_aux p q input []).
   + discriminate.
   + destruct many_until_aux.
     ++ discriminate.
@@ -295,7 +312,6 @@ Proof.
   + inversion equ; subst.
     now apply is_strict in e.
 Qed.
-(* end hide *)
 
 (** ** <<some_until>> *)
 
@@ -317,16 +333,16 @@ Definition some_until {α β} `{Input i t}
 Definition sep {α β} `{Input i t} (p : parser i α)
     (q : parser i β) `{!StrictParser q, !Parser p}
   : parser i (list α) :=
-  cons <$> p <*> many (q *> p).
+  cons <$> p <*> many (q;; p).
 
 (** ** <<eoi>> *)
 
 Definition eoi `{Input i t} : parser i unit :=
-  fun input =>
-    match unpack input with
-    | None => inr (tt, input)
-    | Some (c, _) => inl ["Expected end of input, found " ++ token_to_text c]
-    end.
+  mkStateT (fun input =>
+              match unpack input with
+              | None => inr (tt, input)
+              | Some (c, _) => inl [("Expected end of input, found " ++ token_to_text c)%string]
+              end).
 
 Instance eoi_Parser `(Input i t) : Parser (eoi (i := i)).
 
@@ -334,7 +350,8 @@ Proof.
   constructor.
   intros input res output Heq.
   unfold eoi in Heq.
-  destruct (unpack input) as [[tok in']|]; cbn in *.
+  cbn in *.
+  destruct (unpack input) as [[tok in'] | ]; cbn in *.
   + discriminate.
   + now inversion Heq.
 Qed.
@@ -342,16 +359,17 @@ Qed.
 (** ** <<skip>> *)
 
 Definition skip {i α} (p : parser i α) : parser i unit :=
-  p *> pure tt.
+  p;;
+  pure tt.
 
 (** ** <<peek>> *)
 
 Definition peek {i α} (p : parser i α) : parser i α :=
-  fun input =>
-    match p input with
-    | inr (x, _) => inr (x, input)
-    | inl x => inl x
-    end.
+  mkStateT (fun input =>
+              match runStateT p input with
+              | inr (x, _) => inr (x, input)
+              | inl x => inl x
+              end).
 
 Instance peek_Parser `(Input i t) (a : Type) (p : parser i a) : Parser (peek p).
 
@@ -359,7 +377,8 @@ Proof.
   constructor.
   intros input res output Heq.
   unfold peek in Heq.
-  destruct (p input) as [err | [res' in']]; cbn in *.
+  cbn in *.
+  destruct (runStateT p input) as [err | [res' in']]; cbn in *.
   + discriminate.
   + now inversion Heq.
 Qed.
